Make the function type contractive.
Also, changed the way we substitute lists, so that we do not need to to substitute de function name separately.
Parameters get substituted from right to left.

theories/lang/lang.v
@@ -159,18 +159,17 @@ Definition subst' (mx : binder) (es : expr) : expr → expr :=
 Fixpoint subst_l (xl : list binder) (esl : list expr) (e : expr) : option expr :=
   match xl, esl with
   | [], [] => Some e
-  | x::xl, es::esl => subst_l xl esl (subst' x es e)
+  | x::xl, es::esl => subst' x es <$> subst_l xl esl e
   | _, _ => None
   end.
 
-Definition subst_v (xl : list binder) (esl : vec expr (length xl))
+Definition subst_v (xl : list binder) (vsl : vec val (length xl))
                    (e : expr) : expr :=
-  from_option id (Var "" (* Dummy *)) (subst_l xl esl e).
-Lemma subst_v_eq (xl : list binder) (esl : vec expr (length xl)) e :
-  Some $ subst_v xl esl e = subst_l xl esl e.
+  Vector.fold_right2 (λ b, subst' b ∘ of_val) e _ (list_to_vec xl) vsl.
+Lemma subst_v_eq (xl : list binder) (vsl : vec val (length xl)) e :
+  Some $ subst_v xl vsl e = subst_l xl (of_val <$> vec_to_list vsl) e.
 Proof.
-  unfold subst_v. destruct subst_l eqn:EQ; first done. exfalso. revert esl e EQ.
-  induction xl=>/= esl; inv_vec esl; first done. simpl. eauto.
+  revert vsl. induction xl=>/= vsl; inv_vec vsl=>//=v vsl. by rewrite -IHxl.
 Qed.
 
 (** The stepping relation *)
@@ -230,8 +229,8 @@ Inductive head_step : expr → state → expr → state → list expr → Prop :
 | BetaS f xl e e' el σ:
     Forall (λ ei, is_Some (to_val ei)) el →
     Closed (f :b: xl +b+ []) e →
-    subst_l xl el e = Some e' →
-    head_step (App (Rec f xl e) el) σ (subst' f (Rec f xl e) e') σ []
+    subst_l (f::xl) (Rec f xl e :: el) e = Some e' →
+    head_step (App (Rec f xl e) el) σ e' σ []
 | ReadScS l n v σ:
     σ !! l = Some (RSt n, v) →
     head_step (Read ScOrd (Lit $ LitLoc l)) σ (of_val v) σ []
